More work

theories/DisjointSetUnionCode.v
@@ -7,6 +7,11 @@ Definition state : BlockchainState := fun address =>
     BlockchainContract arrayIndex0 _ (arrayType _ environment0) (arrays _ environment0) 100000%Z (funcdef_0__main (fun x => false) (fun x => 0%Z) (fun x => repeat 0%Z 20))
   else ExternallyOwned 0%Z.
 
+Definition stateAfterInteractions arrays : BlockchainState := fun address =>
+  if decide (address = repeat (0%Z) 20) then
+    BlockchainContract arrayIndex0 _ (arrayType _ environment0) arrays 100000%Z (funcdef_0__main (fun x => false) (fun x => 0%Z) (fun x => repeat 0%Z 20))
+  else ExternallyOwned 0%Z.
+
 Fixpoint interact (state : BlockchainState) (interactions : list (Z * Z)) :=
   match interactions with
   | [] => getBalance (state (repeat 1%Z 20))
@@ -22,6 +27,13 @@ Definition optimalInteractions (x : list (Z * Z)) := forall x', Z.le (interact s
 Inductive Slot :=
 | ReferTo (x : nat)
 | Ancestor (x : Tree).
+
+Fixpoint convertToArray (x : list Slot) : list Z :=
+  match x with
+  | [] => []
+  | (ReferTo x) :: tail => (Z.of_nat x) :: convertToArray tail
+  | (Ancestor x) :: tail => (Z.sub 256%Z (Z.of_nat (leafCount x))) :: convertToArray tail
+  end.
 
 Fixpoint ancestor (dsu : list Slot) (fuel : nat) (index : nat) :=
   match fuel with
@@ -67,4 +79,22 @@ Fixpoint dsuFromInteractions (dsu : list Slot) (interactions : list (nat * nat))
   | (a, b)::tail => dsuFromInteractions (unite dsu a b) tail
   end.
 
-Definition modelScore (interactions : list (Z * Z)) := Z.of_nat (list_sum (map (fun x => match x with | ReferTo _ => 0 | Ancestor x => leafCount x end) (dsuFromInteractions (repeat (Ancestor Unit) 100) (map (fun (x : Z * Z) => let (a, b) := x in (Z.to_nat a, Z.to_nat b)) interactions)))).
+Definition dsuScore (dsu : list Slot) := Z.of_nat (list_sum (map (fun x => match x with | ReferTo _ => 0 | Ancestor x => score x end) dsu)).
+
+Definition dsuLeafCount (dsu : list Slot) := Z.of_nat (list_sum (map (fun x => match x with | ReferTo _ => 0 | Ancestor x => leafCount x end) dsu)).
+
+Definition modelScore (interactions : list (Z * Z)) := dsuScore (dsuFromInteractions (repeat (Ancestor Unit) 100) (map (fun (x : Z * Z) => let (a, b) := x in (Z.to_nat a, Z.to_nat b)) interactions)).
+
+Definition getBalanceInvoke (state : BlockchainState) (communication : list Z) :=
+  match invokeContractAux (repeat 1%Z 20) (repeat 0%Z 20) 0 state state communication 1 with
+  | Some (a, b) => getBalance (b (repeat 1%Z 20))
+  | None => 0%Z
+  end.
+
+Lemma invokeCodeNoNone arrays communication : invokeContractAux (repeat 1%Z 20) (repeat 0%Z 20) 0 (stateAfterInteractions arrays) (stateAfterInteractions arrays) communication 1 <> None.
+Proof.
+Admitted.
+
+Lemma interactEqualsModelScore (x : list (Z * Z)) : interact state x = modelScore x.
+Proof.
+Admitted.
